src/syntax_extension/PulseSugar.fst
@@ -141,6 +141,7 @@ type decl =
       is_rec:bool;
       binders:binders;
       ascription:computation_type;
+      measure:option A.term;
       body:stmt;
       range:rng
     }
@@ -168,7 +169,7 @@ let mk_while guard id invariant body = While { guard; id; invariant; body }
 let mk_intro vprop witnesses = Introduce { vprop; witnesses }
 let mk_sequence s1 s2 = Sequence { s1; s2 }
 let mk_stmt s range = { s; range }
-let mk_fn_decl id is_rec binders ascription body range = FnDecl { id; is_rec; binders; ascription; body; range }
+let mk_fn_decl id is_rec binders ascription measure body range = FnDecl { id; is_rec; binders; ascription; measure; body; range }
 let mk_open lid = Open lid
 let mk_par p1 p2 q1 q2 b1 b2 = Parallel { p1; p2; q1; q2; b1; b2 }
 let mk_rewrite p1 p2 = Rewrite { p1; p2 }
