lib/steel/pulse/Pulse.Recursion.fsti
@@ -7,6 +7,11 @@ open FStar.Tactics.V2
 open Pulse.Syntax
 open Pulse.Typing
 
+val add_knot (g : env)  (rng : R.range)
+             (body : st_term)
+             (nm : string) (nm_orig : string)
+: Tac (s:st_term{Tm_Abs? s.term})
+
 val tie_knot (g : env)  (rng : R.range)
              (body : st_term) (c : comp)
              (nm : string) (nm_orig : string)
